tests/hashmap/Hashmap.Properties.fst
@@ -12,6 +12,46 @@ module InteractiveHelpers = FStar.InteractiveHelpers
 
 #set-options "--z3rlimit 50 --fuel 0 --ifuel 1"
 
+(*** List lemmas *)
+
+val index_append_lem (#a : Type0) (ls0 ls1 : list a) (i : nat{i < length ls0 + length ls1}) :
+  Lemma (
+    (i < length ls0 ==> index (ls0 @ ls1) i == index ls0 i) /\
+    (i >= length ls0 ==> index (ls0 @ ls1) i == index ls1 (i - length ls0)))
+  [SMTPat (index (ls0 @ ls1) i)]
+
+#push-options "--fuel 1"
+let rec index_append_lem #a ls0 ls1 i =
+  match ls0 with
+  | [] -> ()
+  | x :: ls0' ->
+    if i = 0 then ()
+    else index_append_lem ls0' ls1 (i-1)
+#pop-options
+
+// TODO: remove?
+// Returns the index of the value which satisfies the predicate
+val find_index :
+    #a:Type
+  -> f:(a -> Tot bool)
+  -> ls:list a{Some? (find f ls)}
+  -> Tot (i:nat{
+    i < length ls /\
+    begin match find f ls with
+    | None -> False
+    | Some x -> x == index ls i
+    end})
+
+#push-options "--fuel 1"
+let rec find_index #a f ls =
+  match ls with
+  | [] -> assert(False); 0
+  | x :: ls' ->
+    if f x then 0
+    else 1 + find_index f ls'
+#pop-options
+
+
 (*** Lemmas about Primitives *)
 /// TODO: move those lemmas
 
@@ -33,6 +73,7 @@ let rec list_update_index_dif_lem #a ls i x j =
 
 
 (*** Utilities *)
+// TODO: filter the utilities
 
 val find_update:
      #a:Type
@@ -59,6 +100,16 @@ let rec for_allP (f : 'a -> Tot Type0) (l : list 'a) : Tot Type0 =
   match l with
   | [] -> True
   | hd::tl -> f hd /\ for_allP f tl
+
+val for_all_i_aux: #a:Type -> f:(nat -> a -> Tot bool) -> list a -> nat -> Tot bool
+let rec for_all_i_aux (f : nat -> 'a -> Tot bool) (l : list 'a) (i : nat) : Tot bool =
+  match l with
+  | [] -> true
+  | hd::tl -> f i hd && for_all_i_aux f tl (i+1)
+
+val for_all_i: #a:Type -> f:(nat -> a -> Tot bool) -> list a -> Tot bool
+let for_all_i (f : nat -> 'a -> Tot bool) (l : list 'a) : Tot bool =
+  for_all_i_aux f l 0
 
 val pairwise_relP : #a:Type -> pred:(a -> a -> Tot Type0) -> ls:list a -> Tot Type0
 let rec pairwise_relP #a pred ls =
@@ -94,13 +145,16 @@ let fst_is_disctinct (#a : eqtype) (#b : Type0) (p0 : a & b) (p1 : a & b) : Type
 
 (*** Invariants, models *)
 
+(*
 /// "Natural" length function for [list_t]
 /// TODO: remove? we can reason simply with [list_t_v]
 let rec list_t_len (#t : Type0) (ls : list_t t) : nat =
   match ls with
   | ListNil -> 0
   | ListCons _ _ tl -> 1 + list_t_len tl
+*)
 
+(*
 /// "Natural" append function for [list_t]
 /// TODO: remove? we can reason simply with [list_t_v]
 #push-options "--fuel 1"
@@ -110,9 +164,12 @@ let rec list_t_append (#t : Type0) (ls0 ls1 : list_t t) :
   | ListNil -> ls1
   | ListCons x v tl -> ListCons x v (list_t_append tl ls1)
 #pop-options
+*)
 
 /// The "key" type
-type key = usize
+type key : eqtype = usize
+
+type hash : eqtype = usize
 
 type binding (t : Type0) = key & t
 
@@ -127,6 +184,10 @@ let rec list_t_v (#t : Type0) (ls : list_t t) : assoc_list t =
   | ListNil -> []
   | ListCons k v tl -> (k,v) :: list_t_v tl
 
+let list_t_len (#t : Type0) (ls : list_t t) : nat = length (list_t_v ls)
+let list_t_index (#t : Type0) (ls : list_t t) (i : nat{i < list_t_len ls}) : binding t =
+  index (list_t_v ls) i
+
 /// Representation function for the slots.
 /// Rk.: I hesitated to use [concatMap]
 let slots_t_v (#t : Type0) (slots : slots_t t) : assoc_list t =
@@ -136,7 +197,21 @@ let slots_t_v (#t : Type0) (slots : slots_t t) : assoc_list t =
 let hash_map_t_v (#t : Type0) (hm : hash_map_t t) : assoc_list t =
   slots_t_v hm.hash_map_slots
 
+let hash_key (k : key) : hash =
+  Return?.v (hash_key_fwd k)
+
+let hash_mod_key (k : key) (len : usize{len > 0}) : hash =
+  (hash_key k) % len
+
 let same_key (#t : Type0) (k : key) (b : binding t) : bool = fst b = k
+
+// We take a [nat] instead of a [hash] on purpose
+let same_hash_mod_key (#t : Type0) (len : usize{len > 0}) (h : nat) (b : binding t) : bool =
+  hash_mod_key (fst b) len = h
+
+// We take a [nat] instead of a [hash] on purpose
+(*let same_hash (#t : Type0) (h : nat) (b : binding t) : bool = hash_key (fst b) = h *)
+
 let binding_neq (#t : Type0) (b0 b1 : binding t) : bool = fst b0 <> fst b1
 
 let has_same_binding (#t : Type0) (al : assoc_list t) ((k,v) : binding t) : Type0 =
@@ -147,10 +222,32 @@ let has_same_binding (#t : Type0) (al : assoc_list t) ((k,v) : binding t) : Type
 let hash_map_t_mem (#t : Type0) (hm : hash_map_t t) (k : key) : bool =
   existsb (same_key k) (hash_map_t_v hm)
 
-let hash_map_t_find (#t : Type0) (hm : hash_map_t t) (k : key) : option t =
+let hash_map_t_len (#t : Type0) (hm : hash_map_t t) : nat =
+  hm.hash_map_num_entries
+
+let slot_t_v_find (#t : Type0) (k : key) (slot : list (binding t)) : option t =
+  match find (same_key k) slot with
+  | None -> None
+  | Some (_, v) -> Some v
+
+let slot_t_find (#t : Type0) (k : key) (slot : list_t t) : option t =
+  match find (same_key k) (list_t_v slot) with
+  | None -> None
+  | Some (_, v) -> Some v
+
+// This is a simpler version of the "find" function, which captures the essence
+// of what happens.
+let hash_map_t_find
+  (#t : Type0) (hm : hash_map_t t{length hm.hash_map_slots > 0}) (k : key) : option t =
+  let slots = hm.hash_map_slots in
+  let i = hash_mod_key k (length slots) in
+  let slot = index slots i in
+  slot_t_find k slot
+
+(*let hash_map_t_find (#t : Type0) (hm : hash_map_t t) (k : key) : option t =
  match find (same_key k) (hash_map_t_v hm) with
  | None -> None
- | Some (_, v) -> Some v
+ | Some (_, v) -> Some v*)
 
 /// Auxiliary function stating that two associative lists are "equivalent"
 let assoc_list_equiv (#t : Type0) (al0 al1 : assoc_list t) : Type0 =
@@ -159,15 +256,130 @@ let assoc_list_equiv (#t : Type0) (al0 al1 : assoc_list t) : Type0 =
   // And the reverse is true
   for_allP (has_same_binding al0) al1
 
-/// Base invariant for the hashmap (might temporarily be broken at some point)
+// Introducing auxiliary definitions to help deal with the quantifiers
+
+let not_same_keys_at_j_k
+  (#t : Type0) (ls : list_t t) (j:nat{j < list_t_len ls}) (k:nat{k < list_t_len ls}) :
+  Type0 =
+  fst (list_t_index ls j) <> fst (list_t_index ls k)
+
+(*let not_same_keys_at_j_k
+  (#t : Type0) (ls : list_t t) (j:nat{j < list_t_len ls}) (k:nat{k < list_t_len ls}) :
+  Type0 =
+  fst (list_t_index ls j) <> fst (list_t_index ls k)*)
+
+type slot_t_inv_hash_key_f (#t : Type0) (len : usize{len > 0}) (i : usize) (slot : list_t t) =
+  (j:nat{j < list_t_len slot}) ->
+  Lemma (hash_mod_key (fst (list_t_index slot j)) len = i)
+  [SMTPat (hash_mod_key (fst (list_t_index slot j)) len)]
+  
+type slot_t_inv_not_same_keys_f (#t : Type0) (i : usize) (slot : list_t t) =
+     (j:nat{j < list_t_len slot})
+  -> (k:nat{k < list_t_len slot /\ j < k})
+  -> Lemma (not_same_keys_at_j_k slot j k)
+  [SMTPat (not_same_keys_at_j_k slot j k)]
+
+(**)
+
+/// Invariants for the slots
+/// Rk.: making sure the quantifiers instantiations work was painful. As always.
+
+let slot_t_v_inv
+(#t : Type0) (len : usize{len > 0}) (i : usize) (slot : list (binding t)) : bool =
+  // All the bindings are in the proper slot
+  for_all (same_hash_mod_key len i) slot &&
+  // All the keys are pairwise distinct
+  pairwise_rel binding_neq slot
+
+let slot_t_inv (#t : Type0) (len : usize{len > 0}) (i : usize) (slot : list_t t) : bool =
+  // All the bindings are in the proper slot
+  for_all (same_hash_mod_key len i) (list_t_v slot) &&
+  // All the keys are pairwise distinct
+  pairwise_rel binding_neq (list_t_v slot)
+
+(*
+/// Invariants for the slots
+/// Rk.: making sure the quantifiers instantiations work was painful. As always.
+let slot_t_inv (#t : Type0) (len : usize{len > 0}) (i : usize) (slot : list_t t) : Type0 =
+  // All the hashes of the keys are equal to the current hash
+  (forall (j:nat{j < list_t_len slot}).
+    {:pattern (list_t_index slot j)}
+    hash_mod_key (fst (list_t_index slot j)) len = i) /\
+  // All the keys are pairwise distinct
+  (forall (j:nat{j < list_t_len slot}) (k:nat{k < list_t_len slot /\ j < k}).
+    {:pattern not_same_keys_at_j_k slot j k}
+    k <> j ==> not_same_keys_at_j_k slot j k)
+
+/// Helpers to deal with the quantifier proofs
+let slot_t_inv_to_funs
+  (#t : Type0) (len : usize{len > 0}) (i : usize) (slot : list_t t{slot_t_inv len i slot}) :
+  slot_t_inv_hash_key_f len i slot & slot_t_inv_not_same_keys_f i slot =
+  let f : slot_t_inv_hash_key_f len i slot =
+    fun j -> ()
+  in
+  let g : slot_t_inv_not_same_keys_f i slot =
+    fun j k -> ()
+  in
+  (f, g)
+
+let slot_t_inv_from_funs_lem
+  (#t : Type0) (len : usize{len > 0}) (i : usize) (slot : list_t t)
+  (f : slot_t_inv_hash_key_f len i slot)
+  (g : slot_t_inv_not_same_keys_f i slot) :
+  Lemma (slot_t_inv len i slot) =
+  // Dealing with quantifiers is annoying, like always
+  let f' (j:nat{j < list_t_len slot}) :
+    Lemma (hash_mod_key (fst (list_t_index slot j)) len = i)
+    [SMTPat (hash_mod_key (fst (list_t_index slot j)) len)]
+    =
+    f j
+  in
+  let g' (j:nat{j < list_t_len slot}) (k:nat{k < list_t_len slot /\ j < k}) :
+    Lemma (not_same_keys_at_j_k slot j k)
+    [SMTPat (not_same_keys_at_j_k slot j k)]
+    =
+    g j k
+  in
+  ()
+*)
+
+let slots_t_inv (#t : Type0) (slots : slots_t t{length slots <= usize_max}) : Type0 =
+  forall(i:nat{i < length slots}).
+  {:pattern index slots i}
+  slot_t_inv (length slots) i (index slots i)
+
+type slots_t_inv_f (#t : Type0) (slots : slots_t t{length slots <= usize_max}) =
+  (i:nat{i < length slots}) ->
+  Lemma (slot_t_inv (length slots) i (index slots i))
+
+let slots_t_inv_to_fun
+  (#t : Type0) (slots : slots_t t{length slots <= usize_max /\ slots_t_inv slots}) :
+  slots_t_inv_f slots =
+  fun i -> ()
+
+let slots_t_from_fun
+  (#t : Type0) (slots : slots_t t{length slots <= usize_max})
+  (f : slots_t_inv_f slots) :
+  Lemma (slots_t_inv slots) =
+  let f' (i:nat{i < length slots}) :
+    Lemma (slot_t_inv (length slots) i (index slots i))
+    [SMTPat (slot_t_inv (length slots) i (index slots i))]
+    =
+    f i
+  in
+  ()
+
+/// Base invariant for the hashmap (the complete invariant can be temporarily
+/// broken between the moment we inserted an element and the moment we resize)
 let hash_map_t_base_inv (#t : Type0) (hm : hash_map_t t) : Type0 =
   let al = hash_map_t_v hm in
   // [num_entries] correctly tracks the number of entries in the table
+  // Note that it gives us that the length of the slots array is <= usize_max
   hm.hash_map_num_entries = length al /\
-  // All the keys are pairwise distinct
-  pairwise_rel binding_neq al /\
-  // The capacity must be > 0 (otherwise we can't resize, because we multiply
-  // the capacity by two!)
+  // Slots invariant
+  slots_t_inv hm.hash_map_slots /\
+  // The capacity must be > 0 (otherwise we can't resize, because we
+  // multiply the capacity by two!)
   length hm.hash_map_slots > 0 /\
   // Load computation
   begin
@@ -192,58 +404,84 @@ let hash_map_t_is_al (#t : Type0) (hm : hash_map_t t) (al : assoc_list t) : Type
   let hm_al = hash_map_t_v hm in
   assoc_list_equiv hm_al al
 
+(*
 /// The invariant we reveal to the user
 let hash_map_t_inv_repr (#t : Type0) (hm : hash_map_t t) (al : assoc_list t) : Type0 =
   // The hash map invariant is satisfied
   hash_map_t_inv hm /\
   // And it can be seen as the given associative list
   hash_map_t_is_al hm al
-
-let hash_map_len (#t : Type0) (hm : hash_map_t t) : nat =
-  hm.hash_map_num_entries
+*)
 
 (*** Proofs *)
 (**** allocate_slots *)
+
+/// Auxiliary lemma
+val slots_t_all_nil_inv_lem
+  (#t : Type0) (slots : vec (list_t t){length slots <= usize_max}) :
+  Lemma (requires (forall (i:nat{i < length slots}). index slots i == ListNil))
+  (ensures (slots_t_inv slots))
+
+#push-options "--fuel 1"
+let slots_t_all_nil_inv_lem #t slots = ()
+#pop-options
+
+val slots_t_v_all_nil_is_empty_lem
+  (#t : Type0) (slots : vec (list_t t)) :
+  Lemma (requires (forall (i:nat{i < length slots}). index slots i == ListNil))
+  (ensures (slots_t_v slots == []))
+
+#push-options "--fuel 1"
+let rec slots_t_v_all_nil_is_empty_lem #t slots =
+ match slots with
+ | [] -> ()
+ | s :: slots' ->
+   assert(forall (i:nat{i < length slots'}). index slots' i == index slots (i+1));
+   slots_t_v_all_nil_is_empty_lem #t slots';
+   assert(slots_t_v slots == list_t_v s @ slots_t_v slots');
+   assert(slots_t_v slots == list_t_v s);
+   assert(index slots 0 == ListNil)
+#pop-options
+
+/// [allocate_slots]
 val hash_map_allocate_slots_fwd_lem
   (t : Type0) (slots : vec (list_t t)) (n : usize) :
   Lemma
-  (requires (slots_t_v slots == [] /\ length slots + n <= usize_max))
+  (requires (length slots + n <= usize_max))
   (ensures (
    match hash_map_allocate_slots_fwd t slots n with
    | Fail -> False
    | Return slots' ->
-     slots_t_v slots' == [] /\
-     length slots' = length slots + n))
+     length slots' = length slots + n /\
+     // We leave the already allocated slots unchanged
+     (forall (i:nat{i < length slots}). index slots' i == index slots i) /\
+     // We allocate n additional empty slots
+     (forall (i:nat{length slots <= i /\ i < length slots'}). index slots' i == ListNil)))
   (decreases (hash_map_allocate_slots_decreases t slots n))
 
 #push-options "--fuel 1"
 let rec hash_map_allocate_slots_fwd_lem t slots n =
-  if n = 0 then ()
-  else
+  begin match n with
+  | 0 -> ()
+  | _ ->
     begin match vec_push_back (list_t t) slots ListNil with
-    | Fail -> assert(False)
-    | Return v ->
-      (* Prove that the new slots [v] represent an empty mapping *)
-      assert(v == slots @ [ListNil]);
-      map_append list_t_v slots [ListNil];
-      assert(map list_t_v v == map list_t_v slots @ map list_t_v [ListNil]);
-      assert_norm(map (list_t_v #t) [ListNil] == [[]]);
-      flatten_append (map list_t_v slots) [[]];
-      assert(slots_t_v v == slots_t_v slots @ slots_t_v [ListNil]);
-      assert_norm(slots_t_v #t [ListNil] == []);
-      assert(slots_t_v v == slots_t_v slots @ []);
-      assert(slots_t_v v == slots_t_v slots);
-      assert(slots_t_v v == []);
+    | Fail -> ()
+    | Return slots1 ->
       begin match usize_sub n 1 with
-      | Fail -> assert(False)
+      | Fail -> ()
       | Return i ->
-        hash_map_allocate_slots_fwd_lem t v i;
-        begin match hash_map_allocate_slots_fwd t v i with
-        | Fail -> assert(False)
-        | Return v0 -> ()
+        hash_map_allocate_slots_fwd_lem t slots1 i;
+        begin match hash_map_allocate_slots_fwd t slots1 i with
+        | Fail -> ()
+        | Return slots2 ->
+          assert(length slots1 = length slots + 1);
+          assert(slots1 == slots @ [ListNil]); // Triggers patterns
+          assert(index slots1 (length slots) == index [ListNil] 0); // Triggers patterns
+          assert(index slots1 (length slots) == ListNil)
         end
       end
     end
+  end
 #pop-options
 
 (**** new_with_capacity *)
@@ -260,9 +498,18 @@ val hash_map_new_with_capacity_fwd_lem
   (ensures (
     match hash_map_new_with_capacity_fwd t capacity max_load_dividend max_load_divisor with
     | Fail -> False
-    | Return hm -> hash_map_t_inv_repr hm []))
+    | Return hm ->
+      // The hash map has the specified capacity - we need to reveal this
+      // otherwise the pre of [hash_map_t_find] is not satisfied.
+      length hm.hash_map_slots = capacity /\
+      // The hash map has 0 values
+      hash_map_t_len hm = 0 /\
+      // It contains no bindings
+      (forall k. hash_map_t_find hm k == None) /\
+      // We need this low-level property for the invariant
+      (forall(i:nat{i < length hm.hash_map_slots}). index hm.hash_map_slots i == ListNil)))
 
-#push-options "--fuel 1"
+#push-options "--z3rlimit 50 --fuel 1"
 let hash_map_new_with_capacity_fwd_lem (t : Type0) (capacity : usize)
   (max_load_dividend : usize) (max_load_divisor : usize) =
   let v = vec_new (list_t t) in
@@ -278,26 +525,35 @@ let hash_map_new_with_capacity_fwd_lem (t : Type0) (capacity : usize)
       | Fail -> assert(False)
       | Return i0 ->
           let hm = Mkhash_map_t 0 (max_load_dividend, max_load_divisor) i0 v0 in
-          // The base invariant
-          let al = hash_map_t_v hm in
-          assert(hash_map_t_base_inv hm);
-          assert(hash_map_t_inv hm);
-          assert(hash_map_t_is_al hm [])
+          slots_t_all_nil_inv_lem v0
       end
     end
   end
 #pop-options
 
 (**** new *)
-/// [new] doesn't fail and returns an empty hash map.
-val hash_map_new_fwd_lem (t : Type0) :
+/// [new] doesn't fail and returns an empty hash map
+val hash_map_new_fwd_lem_fun (t : Type0) :
   Lemma
   (ensures (
     match hash_map_new_fwd t with
     | Fail -> False
-    | Return hm -> hash_map_t_inv_repr hm []))
+    | Return hm ->
+      // The hash map invariant is satisfied
+      hash_map_t_inv hm /\
+      // The hash map has 0 values
+      hash_map_t_len hm = 0 /\
+      // It contains no bindings
+      (forall k. hash_map_t_find hm k == None)))
 
-let hash_map_new_fwd_lem t = hash_map_new_with_capacity_fwd_lem t 32 4 5
+#push-options "--fuel 1"
+let hash_map_new_fwd_lem_fun t =
+  hash_map_new_with_capacity_fwd_lem t 32 4 5;
+  match hash_map_new_with_capacity_fwd t 32 4 5 with
+  | Fail -> ()
+  | Return hm ->
+    slots_t_v_all_nil_is_empty_lem hm.hash_map_slots
+#pop-options
 
 (**** clear_slots *)
 /// [clear_slots] doesn't fail and simply clears the slots starting at index i
@@ -340,34 +596,9 @@ let rec hash_map_clear_slots_fwd_back_lem
   else ()
 #pop-options
 
-/// Auxiliary lemma:
-/// if all the slots in a vector are [ListNil], then this vector viewed as a list
-/// is empty.
-#push-options "--fuel 1"
-let rec slots_t_v_all_nil_is_empty_lem (#t : Type0) (slots : slots_t t) :
-  Lemma (requires (forall (i:nat{i < length slots}). index slots i == ListNil))
-  (ensures (slots_t_v slots == []))
-  =
-  match slots with
-  | [] -> ()
-  | s :: slots' ->
-    (* The following assert helps the instantiation of quantifiers... *)
-    assert(forall (i:nat{i < length slots'}). index slots' i == index slots (i+1));
-    slots_t_v_all_nil_is_empty_lem slots';
-    assert(slots_t_v slots == flatten (map list_t_v (s :: slots')));
-    assert(slots_t_v slots == flatten (list_t_v s :: map list_t_v slots'));
-    assert(slots_t_v slots == append (list_t_v s) (flatten (map list_t_v slots')));
-    assert(slots_t_v slots == append (list_t_v s) (flatten (map list_t_v slots')));
-    assert(slots_t_v slots == append (list_t_v s) []);
-    assert(slots_t_v slots == (list_t_v s) @ []); // Triggers an SMT pat
-    assert(slots_t_v slots == list_t_v s);
-    assert(index slots 0 == s);
-    assert(slots_t_v slots == [])
-#pop-options
-
 (**** clear *)
 /// [clear] doesn't fail and turns the hash map into an empty map
-val hash_map_clear_fwd_back_lem
+val hash_map_clear_fwd_back_lem_fun
   (t : Type0) (self : hash_map_t t) :
   Lemma
   (requires (hash_map_t_inv self))
@@ -375,11 +606,16 @@ val hash_map_clear_fwd_back_lem
     match hash_map_clear_fwd_back t self with
     | Fail -> False
     | Return hm ->
-      hash_map_t_inv_repr hm []))
+      // The hash map invariant is satisfied
+      hash_map_t_inv hm /\
+      // The hash map has 0 values
+      hash_map_t_len hm = 0 /\
+      // It contains no bindings
+      (forall k. hash_map_t_find hm k == None)))
 
 // Being lazy: fuel 1 helps a lot...
 #push-options "--fuel 1"
-let hash_map_clear_fwd_back_lem t self =
+let hash_map_clear_fwd_back_lem_fun t self =
   let p = self.hash_map_max_load_factor in
   let i = self.hash_map_max_load in
   let v = self.hash_map_slots in
@@ -391,11 +627,9 @@ let hash_map_clear_fwd_back_lem t self =
     let hm1 = Mkhash_map_t 0 p i slots1 in
     assert(hash_map_t_base_inv hm1);
     assert(hash_map_t_inv hm1);
-    assert(hash_map_t_is_al hm1 []);
-    assert(hash_map_t_inv_repr hm1 [])
+    assert(hash_map_t_is_al hm1 [])
   end
 #pop-options
-
 
 (**** len *)
 
@@ -406,14 +640,14 @@ val hash_map_len_fwd_lem (t : Type0) (self : hash_map_t t) :
   Lemma (
     match hash_map_len_fwd t self with
     | Fail -> False
-    | Return l -> l = hash_map_len self)
+    | Return l -> l = hash_map_t_len self)
 
 let hash_map_len_fwd_lem t self = ()
 
 
 (**** insert_in_list *)
 
-/// [insert_in_list_fwd]: returns true iff the key is not in the list
+/// [insert_in_list_fwd]: returns true iff the key is not in the list (functional version)
 val hash_map_insert_in_list_fwd_lem
   (t : Type0) (key : usize) (value : t) (ls : list_t t) :
   Lemma
@@ -421,7 +655,7 @@ val hash_map_insert_in_list_fwd_lem
     match hash_map_insert_in_list_fwd t key value ls with
     | Fail -> False
     | Return b ->
-      b <==> (find (same_key key) (list_t_v ls) == None)))
+      b <==> (slot_t_find key ls == None)))
   (decreases (hash_map_insert_in_list_decreases t key value ls))
 
 #push-options "--fuel 1"
@@ -444,11 +678,227 @@ let rec hash_map_insert_in_list_fwd_lem t key value ls =
   end
 #pop-options
 
+(*
+/// [insert_in_list]
+// TODO: remove
+val hash_map_insert_in_list_back_lem
+  (t : Type0) (len : usize{len > 0}) (key : usize) (value : t) (ls : list_t t) :
+  Lemma
+  (requires (slot_t_inv len (hash_mod_key key len) ls))
+  (ensures (
+    match hash_map_insert_in_list_back t key value ls with
+    | Fail -> False
+    | Return ls' ->
+      // The invariant is preserved
+      slot_t_inv len (hash_mod_key key len) ls' /\
+      // [key] maps to [value]
+      slot_t_find key ls' == Some value /\
+      // The other bindings are preserved
+      (forall k'. k' <> key ==> slot_t_find k' ls' == slot_t_find k' ls) /\
+      // The length is incremented, iff we inserted a new key
+      (match slot_t_find key ls with
+       | None ->
+         list_t_v ls' == list_t_v ls @ [(key,value)] /\
+         list_t_len ls' = list_t_len ls + 1
+       | Some _ ->
+         list_t_v ls' == find_update (same_key key) (list_t_v ls) (key,value) /\
+         list_t_len ls' = list_t_len ls)))
+  (decreases (hash_map_insert_in_list_decreases t key value ls))
+
+// I suffered a bit below, but as usual, for the wrong reasons: quantifiers in F*
+// are really too painful to work with...
+#push-options "--z3rlimit 200 --fuel 1"
+let rec hash_map_insert_in_list_back_lem t len key value ls =
+  let h = hash_mod_key key len in
+  begin match ls with
+  | ListCons ckey cvalue ls0 ->
+    let b = ckey = key in
+    if b
+    then
+      begin
+      let ls1 = ListCons ckey value ls0 in
+      let ls_hash_key_lem, ls_not_same_keys_lem = slot_t_inv_to_funs len h ls in
+      let ls1_hash_key_lem : slot_t_inv_hash_key_f len h ls1 =
+        fun j -> if j = 0 then () else ls_hash_key_lem j
+      in
+      let ls1_not_same_keys_lem : slot_t_inv_not_same_keys_f h ls1 =
+        fun j k -> ls_not_same_keys_lem j k
+      in
+      slot_t_inv_from_funs_lem len h ls1 ls1_hash_key_lem ls1_not_same_keys_lem;
+      assert(slot_t_inv len (hash_mod_key key len) ls1)
+      end
+    else
+      begin
+      let ls_hash_key_lem, ls_not_same_keys_lem = slot_t_inv_to_funs len h ls in
+      let ls0_hash_key_lem : slot_t_inv_hash_key_f len h ls0 =
+        fun j -> ls_hash_key_lem (j + 1)
+      in
+      let ls0_not_same_keys_lem : slot_t_inv_not_same_keys_f h ls0 =
+        fun j k -> ls_not_same_keys_lem (j + 1) (k + 1)
+      in
+      slot_t_inv_from_funs_lem len h ls0 ls0_hash_key_lem ls0_not_same_keys_lem;
+      assert(slot_t_inv len (hash_mod_key key len) ls0);
+      hash_map_insert_in_list_back_lem t len key value ls0;
+      match hash_map_insert_in_list_back t key value ls0 with
+      | Fail -> ()
+      | Return l ->
+        let ls1 = ListCons ckey cvalue l in
+        let l_hash_key_lem, l_not_same_keys_lem = slot_t_inv_to_funs len h l in
+        let ls1_hash_key_lem : slot_t_inv_hash_key_f len h ls1 =
+          fun j ->
+          if j = 0 then
+            begin
+            ls_hash_key_lem 0;
+            assert(hash_mod_key (fst (list_t_index ls1 j)) len = h)
+            end
+          else l_hash_key_lem (j - 1)
+        in
+        (* Disjunction on whether we added an element or not *)
+        begin match slot_t_find key ls0 with
+        | None ->
+          (* We added an element *)        
+          assert(list_t_v l == list_t_v ls0 @ [(key,value)]);
+  //        assert(list_t_v ls1 == list_t_v ls @ [(key,value)]);
+          let ls1_not_same_keys_lem : slot_t_inv_not_same_keys_f h ls1 =
+            fun j k ->
+            if 0 < j then
+              l_not_same_keys_lem (j-1) (k-1)
+            else //if k < list_t_len ls then
+              begin
+//              assert_norm(length [(key,value)] = 1);
+              assert(list_t_index ls1 j == (ckey, cvalue));
+              assert(list_t_v ls1 == (ckey, cvalue) :: list_t_v l);
+              assert(list_t_index ls1 k == list_t_index l (k-1));
+//              index_append_lem (list_t_v ls0) [(key,value)] (j-1);
+              index_append_lem (list_t_v ls0) [(key,value)] (k-1);
+              if k < list_t_len l then
+                begin
+                assert(list_t_index ls1 k == list_t_index ls0 (k-1));
+                admit()
+                end
+              else
+                admit()
+              end
+          in
+          slot_t_inv_from_funs_lem len h ls1 ls1_hash_key_lem ls1_not_same_keys_lem
+        | _ ->
+          (* We simply updated a binding *)
+          admit()
+        end
+      end
+  | ListNil ->
+    let ls0 = ListCons key value ListNil in
+    assert_norm(list_t_len ls0 == 1);
+    let ls0_hash_key_lem : slot_t_inv_hash_key_f len h ls0 =
+      fun j -> ()
+    in
+    let ls0_not_same_keys_lem : slot_t_inv_not_same_keys_f h ls0 =
+      fun j k -> ()
+    in
+    slot_t_inv_from_funs_lem len h ls0 ls0_hash_key_lem ls0_not_same_keys_lem
+  end
+#pop-options
+*)
+
+(**** insert_no_resize *)
+
+(*val hash_map_insert_no_resize_fwd_back_lem
+  (t : Type0) (self : hash_map_t t) (key : usize) (value : t) :
+  Lemma (requires (hash_map_t_inv self))
+  (ensures (
+    match hash_map_insert_no_resize_fwd_back t self key value with
+    | Fail ->
+      (* If we fail, it is necessarily because:
+       * - we tried to add a new *key* (there was no binding for the key)
+       * - the [num_entries] counter is already saturaed *)
+      hash_map_t_find self key == None /\
+      hash_map_t_len self = usize_max
+    | Return hm ->
+      // The invariant is preserved
+      hash_map_t_inv hm /\
+      // [key] maps to [value]
+      hash_map_t_find hm key == Some value /\
+      // The other bindings are preserved
+      (forall k'. k' <> key ==> hash_map_t_find hm k' == hash_map_t_find self k') /\
+      // The length is incremented, iff we inserted a new key
+      (match hash_map_t_find self key with
+       | None -> hash_map_t_len hm = hash_map_t_len hm + 1
+       | Some _ -> hash_map_t_len hm = hash_map_t_len hm)))
+
+let hash_map_insert_no_resize_fwd_back_lem t self key value =
+  begin match hash_key_fwd key with
+  | Fail -> ()
+  | Return i ->
+    let i0 = self.hash_map_num_entries in
+    let p = self.hash_map_max_load_factor in
+    let i1 = self.hash_map_max_load in
+    let v = self.hash_map_slots in
+    let i2 = vec_len (list_t t) v in
+    begin match usize_rem i i2 with
+    | Fail -> ()
+    | Return hash_mod ->
+      begin match vec_index_mut_fwd (list_t t) v hash_mod with
+      | Fail -> ()
+      | Return l ->
+        begin
+        hash_map_insert_in_list_fwd_lem t key value l;
+        match hash_map_insert_in_list_fwd t key value l with
+        | Fail -> ()
+        | Return b ->
+          if b
+          then
+            begin match usize_add i0 1 with
+            | Fail ->
+              assert(slot_t_find key l == None);
+              assert(hash_map_t_len self = usize_max);
+              ()
+            | Return i3 ->
+              assert(l == index v hash_mod);
+              slots_t_inv_to_fun v hash_mod;
+              assert(slot_t_inv hash_mod (index v hash_mod));
+              assert(slot_t_inv (hash_key key) l);
+              hash_map_insert_in_list_back_lem t key value l;
+              begin match hash_map_insert_in_list_back t key value l with
+              | Fail -> admit()
+              | Return l0 ->
+                begin match vec_index_mut_back (list_t t) v hash_mod l0 with
+                | Fail -> admit()
+                | Return v0 ->
+                  let self0 = Mkhash_map_t i3 p i1 v0 in admit() //Return self0
+                end
+              end
+            end
+          else
+            begin match hash_map_insert_in_list_back t key value l with
+            | Fail -> admit()
+            | Return l0 ->
+              begin match vec_index_mut_back (list_t t) v hash_mod l0 with
+              | Fail -> admit()
+              | Return v0 ->
+                let self0 = Mkhash_map_t i0 p i1 v0 in admit() //Return self0
+              end
+            end
+        end
+      end
+    end
+  end*)
+
 /// The proofs about [insert_in_list] backward are easier to do in several steps:
 /// extrinsic proofs to the rescue!
+/// Rk.: those proofs actually caused a lot of trouble because:
+/// - F* is extremely bad at reasoning with quantifiers, which is made worse by
+///   the fact we are blind when making proofs. This forced us to be extremely
+///   careful about the way we wrote our specs/invariants (by writing "functional"
+///   specs and invariants, mostly, so as not to manipulate quantifiers)
+/// - we can't easily prove intermediate results which require a recursive proofs
+///   inside of other proofs, meaning that whenever we need such a result we need
+///   to write an intermediate lemma, which is extremely cumbersome.
+/// Note that in a theorem prover with tactics, most of the below proof would have
+/// been extremely straightforward. In particular, we wouldn't have needed to think
+/// much about the invariants, nor to cut the proofs into very small, modular lemmas.
 
-/// [insert_in_list]: if the key is not in the map, appends a new bindings
-val hash_map_insert_in_list_back_lem_append
+/// [insert_in_list]: if the key is not in the map, appends a new bindings (functional version)
+val hash_map_insert_in_list_back_lem_append_fun
   (t : Type0) (key : usize) (value : t) (ls : list_t t) :
   Lemma
   (requires (
@@ -461,15 +911,15 @@ val hash_map_insert_in_list_back_lem_append
   (decreases (hash_map_insert_in_list_decreases t key value ls))
 
 #push-options "--fuel 1"
-let rec hash_map_insert_in_list_back_lem_append t key value ls =
+let rec hash_map_insert_in_list_back_lem_append_fun t key value ls =
   begin match ls with
   | ListCons ckey cvalue ls0 ->
     let b = ckey = key in
     if b
-    then () //let ls1 = ListCons ckey value ls0 in Return ls1
+    then ()
     else
       begin
-      hash_map_insert_in_list_back_lem_append t key value ls0;
+      hash_map_insert_in_list_back_lem_append_fun t key value ls0;
       match hash_map_insert_in_list_back t key value ls0 with
       | Fail -> ()
       | Return l -> ()
@@ -478,8 +928,8 @@ let rec hash_map_insert_in_list_back_lem_append t key value ls =
   end
 #pop-options
 
-/// [insert_in_list]: if the key is in the map, we update the binding
-val hash_map_insert_in_list_back_lem_update
+/// [insert_in_list]: if the key is in the map, we update the binding (functional version)
+val hash_map_insert_in_list_back_lem_update_fun
   (t : Type0) (key : usize) (value : t) (ls : list_t t) :
   Lemma
   (requires (
@@ -492,7 +942,7 @@ val hash_map_insert_in_list_back_lem_update
   (decreases (hash_map_insert_in_list_decreases t key value ls))
 
 #push-options "--fuel 1"
-let rec hash_map_insert_in_list_back_lem_update t key value ls =
+let rec hash_map_insert_in_list_back_lem_update_fun t key value ls =
   begin match ls with
   | ListCons ckey cvalue ls0 ->
     let b = ckey = key in
@@ -500,7 +950,7 @@ let rec hash_map_insert_in_list_back_lem_update t key value ls =
     then ()
     else
       begin
-      hash_map_insert_in_list_back_lem_update t key value ls0;
+      hash_map_insert_in_list_back_lem_update_fun t key value ls0;
       match hash_map_insert_in_list_back t key value ls0 with
       | Fail -> ()
       | Return l -> ()
@@ -509,6 +959,84 @@ let rec hash_map_insert_in_list_back_lem_update t key value ls =
   end
 #pop-options
 
+/// Auxiliary lemmas
+/// Reasoning about the result of [insert_in_list], converted to a "regular" list.
+/// Note that in F* we can't have recursive proofs inside of other proofs, contrary
+/// to Coq, which makes it a bit cumbersome to prove auxiliary results like the
+/// following ones...
+
+val slot_t_v_for_all_binding_neq_append_lem
+  (t : Type0) (key : usize) (value : t) (ls : list (binding t)) (b : binding t) :
+  Lemma
+  (requires (
+    fst b <> key /\
+    for_all (binding_neq b) ls /\
+    slot_t_v_find key ls == None))
+  (ensures (
+    for_all (binding_neq b) (ls @ [(key,value)])))
+
+#push-options "--fuel 1"
+let rec slot_t_v_for_all_binding_neq_append_lem t key value ls b =
+  match ls with
+  | [] -> ()
+  | (ck, cv) :: cls ->
+    slot_t_v_for_all_binding_neq_append_lem t key value cls b
+#pop-options
+
+val slot_t_v_inv_not_find_append_end_inv_lem
+  (t : Type0) (len : usize{len > 0}) (key : usize) (value : t) (ls : list (binding t)) :
+  Lemma
+  (requires (
+    slot_t_v_inv len (hash_mod_key key len) ls /\
+    slot_t_v_find key ls == None))
+  (ensures (
+    let ls' = ls @ [(key,value)] in
+    slot_t_v_inv len (hash_mod_key key len) ls' /\
+    (slot_t_v_find key ls' == Some value) /\
+    (forall k'. k' <> key ==> slot_t_v_find k' ls' == slot_t_v_find k' ls)))
+
+#push-options "--fuel 1"
+let rec slot_t_v_inv_not_find_append_end_inv_lem t len key value ls =
+  match ls with
+  | [] -> ()
+  | (ck, cv) :: cls ->
+    slot_t_v_inv_not_find_append_end_inv_lem t len key value cls;
+    let h = hash_mod_key key len in
+    let ls' = ls @ [(key,value)] in
+    assert(for_all (same_hash_mod_key len h) ls');
+    slot_t_v_for_all_binding_neq_append_lem t key value cls (ck, cv);
+    assert(pairwise_rel binding_neq ls');
+    assert(slot_t_v_inv len h ls')
+#pop-options
+
+/// [insert_in_list]: if the key is not in the map, appends a new bindings (quantifiers)
+val hash_map_insert_in_list_back_lem_append
+  (t : Type0) (len : usize{len > 0}) (key : usize) (value : t) (ls : list_t t) :
+  Lemma
+  (requires (
+    slot_t_inv len (hash_mod_key key len) ls /\
+    find (same_key key) (list_t_v ls) == None))
+  (ensures (
+    match hash_map_insert_in_list_back t key value ls with
+    | Fail -> False
+    | Return ls' ->
+      list_t_v ls' == list_t_v ls @ [(key,value)] /\
+      // The invariant is preserved
+      slot_t_inv len (hash_mod_key key len) ls' /\
+      // [key] maps to [value]
+      slot_t_find key ls' == Some value /\
+      // The other bindings are preserved
+      (forall k'. k' <> key ==> slot_t_find k' ls' == slot_t_find k' ls)))
+
+let hash_map_insert_in_list_back_lem_append t len key value ls =
+  hash_map_insert_in_list_back_lem_append_fun t key value ls;
+  match hash_map_insert_in_list_back t key value ls with
+  | Fail -> ()
+  | Return ls' ->
+    assert(list_t_v ls' == list_t_v ls @ [(key,value)]);
+    slot_t_v_inv_not_find_append_end_inv_lem t len key value (list_t_v ls)
+
+(*
 (**** insert_no_resize *)
 
 /// Same as for [insert_in_list]: we do the proofs in several, modular steps.
